complete list refactor

FormalizationOfComputability/PhiSeq.lean
@@ -20,94 +20,36 @@ open Nat.Partrec
 open Nat.Partrec.Code
 open List --hiding isSome_getElem?
 
-
-/- The elements whose computations first halt at stage s. By definition,
-these elements are less than s. -/
-def ϕNew (e s : ℕ) : Finset ℕ := (W_s e s).filter (λ n ↦ ϕ_s e (s-1) n = Option.none)
-
-instance ϕNew_dec (e s n : ℕ) : Decidable (n ∈ ϕNew e s) := by
-  exact Finset.decidableMem n (ϕNew e s)
-
-lemma ϕNew_zero (e : ℕ) : ϕNew e 0 = ∅ := by simp [ϕNew]
-
 variable {e s t n x y i k l : ℕ}
-
-/- This lemma cleans up lines that would otherwise be a rather lengthy simp only -/
-lemma ϕNew_mem : x ∈ ϕNew e s ↔ (x < s ∧ ϕ_s_halts e s x ∧ ¬ϕ_s_halts e (s - 1) x) := by
-  simp [ϕNew, ϕ_s_halts]
-  intro h h1
-  exact ϕ_input_bound h
-
-/- The elements newly halting at stage s are exactly W_{e, s} \ W_{e, s-1} -/
-@[grind =]
-lemma ϕNew_eq_Ws_diff : (ϕNew e s) = (W_s e s) \ (W_s e (s-1)) := by
-  apply subset_antisymm
-  · intro x
-    simp_all [ϕNew]
-  · intro x
-    simp_all only [ϕNew]
-    intro h
-    simp only [Finset.mem_filter]
-    simp_all
 
 /- Elements never enter twice - the ϕNew are disjoint -/
 lemma ϕNew_disjoint_gt (h : s > t) : Disjoint (ϕNew e s) (ϕNew e t) := by
-  rw [Finset.disjoint_iff_ne]
-  intros a ha b hb
-  have ⟨d, hd⟩ := Nat.exists_eq_add_of_lt h
-  have hb1 : b ∈ W_s e (t+d) := by
-    apply (W_s_mono (Nat.le_add_right t d))
-    rw [ϕNew_eq_Ws_diff, Finset.mem_sdiff] at hb
-    exact hb.left
-  grind
+  refine disjoint_left.mpr ?_
+  simp_rw [ϕNew_mem]
+  intro a ⟨_, has1⟩ ⟨hat, _⟩
+  exact Ne.elim has1 (ϕ_halts_mono (le_sub_one_of_lt h) hat)
 
-lemma ϕNew_pairwise_disjoint (e : ℕ) : Set.PairwiseDisjoint (Set.univ : Set ℕ) (ϕNew e) := by
-  intro s _ t _ h
-  rw [ne_iff_lt_or_gt] at h
-  rcases h with h | h
-  · exact Disjoint.symm (ϕNew_disjoint_gt h)
-  · exact ϕNew_disjoint_gt h
-
-/- If x is new at stage s, it is not in W_s (elements entering *before* s)-/
-lemma ϕNew_is_new (e s : ℕ) : (ϕNew e s) ∩ (W_s e (s-1)) = ∅ := by simp [ϕNew_eq_Ws_diff]
+lemma ϕNew_pairwise_disjoint (h : s ≠ t) : Disjoint (ϕNew e s) (ϕNew e t) := by
+  replace h := Nat.lt_or_gt_of_ne h
+  apply Or.elim h
+  <;> intro h1
+  · exact List.Disjoint.symm (ϕNew_disjoint_gt h1)
+  · exact ϕNew_disjoint_gt h1
 
 /- It is sometimes useful to work with W_{e,s} instead of W_{e, s+1} -/
-lemma Ws_eq (e s : ℕ) : W_s e s = (W_s e (s-1)) ∪ (ϕNew e s) := by
-    rw [ϕNew_eq_Ws_diff]
-    simp only [Finset.union_sdiff_self_eq_union, Finset.right_eq_union]
-    apply W_s_mono
-    simp only [tsub_le_iff_right, le_add_iff_nonneg_right, _root_.zero_le]
-
-/- The new elements at stage s are exactly those with runtime s -/
-lemma ϕNew_runtime_iff (e x r : ℕ) : x ∈ ϕNew e r ↔ r ∈ runtime e x := by
-  simp only [runtime, ϕNew_eq_Ws_diff, Finset.mem_sdiff, Part.coe_some, mem_rfind,
-    Part.mem_some_iff, Bool.true_eq, Bool.false_eq, Option.isSome_eq_false_iff,
-    Option.isNone_iff_eq_none]
-  constructor
-  <;> intro ⟨h, h1⟩
-  <;> constructor
-  · exact W_s_ϕ_s.mp h
-  · intro m hm
-    contrapose h1
-    exact W_s_mono (le_sub_one_of_lt hm) (W_s_ϕ_s.mpr (Option.isSome_iff_ne_none.mpr h1))
-  · exact W_s_ϕ_s.mpr h
-  · by_cases hr : r = 0
-    · simp [hr]
-    · have h2 : r-1 < r := by exact Nat.sub_one_lt hr
-      simp_all
+lemma Ws_eq : Ws e s = (Ws e (s-1)) ++ (ϕNew e s) := by
+  cases s with | zero => simp [ϕNew] | succ s => simp [Ws]
 
 /- W_e can be created as a disjoint union of new elements-/
-lemma We_eq_union_ϕNew (e : ℕ) : W e = ⋃ s, (ϕNew e s) := by
-  rw [W_eq_union_W_s]
+lemma We_eq_union_ϕNew : W e = ⋃ s, (ϕNew e s).toFinset := by
+  rw [W_eq_union_Ws]
   apply subset_antisymm
   <;> intro x h
-  <;> simp_all only [Set.mem_iUnion, Finset.mem_coe]
-  · obtain ⟨_, h⟩ := h
-    apply Ws_runtime at h
-    obtain ⟨r, h⟩ := h
-    simp only [ϕNew_runtime_iff]
-    exact ⟨r, h.left⟩
-  · grind
+  <;> simp_all only [Set.mem_iUnion, Finset.mem_coe, mem_toFinset]
+  <;> replace ⟨s, h⟩ := h
+  · replace ⟨r, h⟩ := Ws_runtime h
+    exact ⟨r, ((ϕNew_runtime e x r).mpr h.right.left)⟩
+  · exact ⟨s, Ws_mem.mpr (ϕNew_mem.mp h).left⟩
 
 /- TFAE :
 Eventually all ϕNew e s = ∅
@@ -116,24 +58,25 @@ There is an s such that W_e = W_{e, s}
 -/
 
 /- TODO : Move any implications not needed for lemmas to the TFAE -/
-lemma ϕNew_stabilizes_implies_We_finite (e s : ℕ) (h : ∀ t > s, ϕNew e t = ∅) :
+/- If all large enough ϕNew are empty, then W e is finite. -/
+lemma ϕNew_stabilizes_We_finite (h : ∀ t > s, ϕNew e t = ∅) :
     (W e).Finite := by
   rw [We_eq_union_ϕNew, Set.finite_iUnion_iff]
   · simp only [Finset.finite_toSet, implies_true, Finset.coe_nonempty, true_and]
     apply Set.Finite.subset (Set.finite_le_nat s)
-    grind
-  · simp only [Finset.disjoint_coe]
+    refine Set.setOf_subset_setOf_of_imp ?_
+    simp only [toFinset_nonempty_iff, ne_eq]
+    exact fun a a_1 ↦ Nat.le_of_not_lt fun a_2 ↦ a_1 (h a a_2)
+  · simp only [Finset.disjoint_coe, disjoint_toFinset_iff_disjoint]
     intro i j h1
-    apply ϕNew_pairwise_disjoint
-    <;> simp only [Set.mem_univ, ne_eq]
-    exact h1
+    exact ϕNew_pairwise_disjoint h1
 
-lemma We_finite_implies_ϕNew_stabilizes (e : ℕ) (h : (W e).Finite) :
+/- If W e is finite, then all large enough ϕNew are empty. -/
+lemma We_finite_ϕNew_stabilizes (h : (W e).Finite) :
     ∃ s, ∀ t > s, ϕNew e t = ∅ := by
   rw [We_eq_union_ϕNew, Set.finite_iUnion_iff] at h
   simp only [Finset.finite_toSet, implies_true, Finset.coe_nonempty, true_and] at h
-  have h1 := Set.Finite.exists_finset h
-  obtain ⟨P, h1⟩ := h1
+  obtain ⟨P, h1⟩ := Set.Finite.exists_finset h
   · by_cases h2 : P = ∅
     · use 0
       simp_all
@@ -142,97 +85,52 @@ lemma We_finite_implies_ϕNew_stabilizes (e : ℕ) (h : (W e).Finite) :
       contrapose h3
       simp only [gt_iff_lt, Finset.max'_lt_iff, not_forall, not_lt]
       use s
-      grind
+      constructor
+      · rfl
+      · rw [h1 s]
+        simp
+        exact h3
   · simp only [Finset.disjoint_coe]
     intro i j h1
-    apply ϕNew_pairwise_disjoint
-    <;> simp only [Set.mem_univ, ne_eq]
-    exact h1
+    simp only [disjoint_toFinset_iff_disjoint]
+    exact ϕNew_pairwise_disjoint h1
 
-lemma We_finite_iff_ϕNew_stabilizes (e : ℕ) :
-    (W e).Finite ↔ (∃ t, ∀ s > t, ϕNew e s = ∅) := by
+/- W e is finite iff all large enough ϕNew are empty. -/
+lemma We_finite_iff_ϕNew_stabilizes : (W e).Finite ↔ (∃ t, ∀ s > t, ϕNew e s = ∅) := by
   constructor
-  · exact We_finite_implies_ϕNew_stabilizes e
+  · exact We_finite_ϕNew_stabilizes
   · intro ⟨_, h⟩
-    exact ϕNew_stabilizes_implies_We_finite _ _ h
-
-def ϕNewList (e s : ℕ):= (ϕNew e s).sort
-
-instance ϕNewList_dec (e s n : ℕ) : Decidable (n ∈ ϕNewList e s) := by
-  simp_rw [← mem_toFinset]
-  apply Finset.decidableMem
-
-/- The elements in W_e enumerated up to stage s, in the order they appeared. Elements halting
-at the same time are enumerated in asceding order. -/
-def WPrefix (e : ℕ) : ℕ → List ℕ
-    | 0     => []
-    | s + 1 => (WPrefix e s) ++ ϕNewList e (s+1)
-
-/- WPrefix e s is exactly W_{e, s} in order of enumeration -/
-lemma Ws_eq_prefix (e s : ℕ) : W_s e s = (WPrefix e s).toFinset := by
-  induction s with | zero | succ s hs
-  · exact Finset.val_inj.mp rfl
-  · rw [Ws_eq]
-    unfold WPrefix ϕNewList
-    simp_all only [W_s, add_tsub_cancel_right, toFinset_append, Finset.sort_toFinset]
-
-instance WPrefix_dec (e s n : ℕ) : Decidable (n ∈ WPrefix e s) := by
-  simp_rw [← mem_toFinset]
-  apply Finset.decidableMem
-
-/- Elements cannot be enumerated twice-/
-lemma nodup_WPrefix (e s : ℕ) : Nodup (WPrefix e s) := by
-  induction s with | zero | succ s ih
-  · simp [WPrefix]
-  · simp only [WPrefix, ϕNewList]
-    apply List.Nodup.append ih
-    · simp only [Finset.sort_nodup]
-    · rw [ϕNew_eq_Ws_diff]
-      simp only [add_tsub_cancel_right]
-      refine disjoint_left.mpr ?_
-      intro a ha
-      simp only [Finset.mem_sort, Finset.mem_sdiff, not_and]
-      intro hb
-      simp_all only [Ws_eq_prefix, mem_toFinset, not_not]
-
-/- The WPrefixes are prefixes of each other-/
-lemma WPrefix_mono (e s t : ℕ) (h : s ≤ t) :
-  (WPrefix e s) <+: (WPrefix e t) := by
-  induction t with | zero | succ t ih
-  · simp only [nonpos_iff_eq_zero] at h
-    rw [h]
-  · by_cases h1 : s = t + 1
-    · rw [h1]
-    · apply List.IsPrefix.trans (ih (le_of_lt_succ (lt_of_le_of_ne h h1)))
-      simp [WPrefix]
+    exact ϕNew_stabilizes_We_finite h
 
 /- It is often useful to view elements entering one at a time, so there may be a queue
 of elements waiting to enter. This represents the elements still waiting *at* stage s,
 i.e. the head of this list will be enumerated at stage s. -/
 def enter_queue (e : ℕ) : ℕ → List ℕ
   | 0 => []
-  | s + 1 => (enter_queue e s).tail ++ (ϕNew e (s+1)).sort
+  | s + 1 => (enter_queue e s).tail ++ (ϕNew e (s+1))
 
-instance enter_queue_dec (e s n : ℕ) : Decidable (n ∈ enter_queue e s) := by
-  simp_rw [← mem_toFinset]
-  apply Finset.decidableMem
+open Primrec
 
-instance enter_queue_comp (e : ℕ) : Computable (enter_queue e) := by
-  unfold Computable
-  sorry
-
+lemma enter_queue_primrec (e : ℕ) : Primrec (enter_queue e) := by
+  have hstep : Primrec₂ (fun (s : ℕ) (L : List ℕ) => L.tail ++ ϕNew e (s + 1)) := by
+    refine Primrec.list_append.comp₂ ?_ ?_
+    · exact ((Primrec.list_tail : Primrec (fun L : List ℕ => L.tail)).comp Primrec₂.right)
+    · exact (ϕNew_primrec e).comp (Primrec.succ.comp Primrec₂.left)
+  refine (Primrec.nat_rec₁ ([] : List ℕ) hstep).of_eq ?_
+  intro s
+  induction s with
+  | zero => rfl
+  | succ s ih => simp [enter_queue, ih]
 
 /- If n is in the queue at stage s, then ϕ_{e, s}(n)↓ -/
-lemma enter_queue_halts (h : n ∈ enter_queue e s) : ϕ_s_halts e s n := by
+lemma enter_queue_halts (h : n ∈ enter_queue e s) : ϕs_halts e s n := by
   induction s with | zero | succ s ih
   · tauto
   · simp only [enter_queue, List.mem_append] at h
     cases h with | inl h | inr h
-    · apply List.mem_of_mem_tail at h
-      apply ih at h
-      exact ϕ_halts_mono (Nat.le_add_right s 1) h
-    · simp_all only [ϕ_s_halts, Finset.mem_sort, ϕNew_mem, add_tsub_cancel_right,
-      Bool.not_eq_true, Option.isSome_eq_false_iff, Option.isNone_iff_eq_none]
+    · exact ϕ_halts_mono (Nat.le_add_right s 1) (ih (List.mem_of_mem_tail h))
+    · simp_all only [ϕs_halts, ϕNew_mem, add_tsub_cancel_right, Bool.not_eq_true,
+      Option.isSome_eq_false_iff, Option.isNone_iff_eq_none]
 
 /- Elements of the queue are exactly the elements that halt -/
 lemma enter_queue_mem (e n : ℕ) : (∃ s, n ∈ enter_queue e s) ↔ ϕ_halts e n := by
@@ -242,7 +140,7 @@ lemma enter_queue_mem (e n : ℕ) : (∃ s, n ∈ enter_queue e s) ↔ ϕ_halts 
     apply (ϕ_complete).mpr
     use s
   · intro h
-    simp only [ϕ_halts_runtime_exists, ← ϕNew_runtime_iff] at h
+    simp only [ϕ_halts_runtime_exists, ← ϕNew_runtime] at h
     obtain ⟨r, h⟩ := h
     use r
     unfold enter_queue
@@ -253,9 +151,9 @@ lemma enter_queue_mem (e n : ℕ) : (∃ s, n ∈ enter_queue e s) ↔ ϕ_halts 
       simp [h]
 
 /- A lemma for moving from (enter_queue e s) to (enter_queue e t) -/
-lemma enter_queue_ϕNewList (e : ℕ) (h : s ≥ t) :
+lemma enter_queue_ϕNew (e : ℕ) (h : s ≥ t) :
     (enter_queue e s) ⊆
-    (enter_queue e t) ++ flatten ((range (s - t)).map (λ i ↦ ϕNewList e (t + i + 1))) := by
+    (enter_queue e t) ++ flatten ((range (s - t)).map (λ i ↦ ϕNew e (t + i + 1))) := by
   apply Nat.exists_eq_add_of_le at h
   obtain ⟨k, h⟩ := h
   revert s
@@ -278,28 +176,27 @@ lemma enter_queue_ϕNewList (e : ℕ) (h : s ≥ t) :
       refine mem_flatten.mpr ?_
       simp
       use k
-      simp [ϕNewList, xh]
+      simp [xh]
 
-/- The queue at stage s is a suffix of WPrefix e s.
+/- The queue at stage s is a suffix of Ws e s.
 This is mostly here so that it's easy to show that enter queues have no duplicates -/
-lemma enter_queue_WPrefix (e s : ℕ) :
-    IsSuffix (enter_queue e s) (WPrefix e s) := by
+lemma enter_queue_Ws (e s : ℕ) :
+    IsSuffix (enter_queue e s) (Ws e s) := by
   induction s with | zero | succ s ih
-  · simp [enter_queue]
-  · unfold enter_queue WPrefix
+  · simp only [enter_queue, nil_suffix]
+  · unfold enter_queue Ws
     have h1 := List.IsSuffix.trans (tail_suffix (enter_queue e s)) ih
     cases L : (enter_queue e s) with | nil | cons a T
-    · exact suffix_append (WPrefix e s) ((ϕNew e (s + 1)).sort fun a b ↦ a ≤ b)
-    · simp [IsSuffix, L, tail_cons] at h1
+    · simp only [tail_nil, nil_append, suffix_append]
+    · simp only [IsSuffix, L, tail_cons] at h1
       obtain ⟨S, h1⟩ := h1
       use S
-      simp [← h1]
-      exact toList_toArray
+      simp only [tail_cons, ← h1, append_assoc]
 
 /- The queues have no duplicates. -/
 lemma enter_queue_nodup (e s : ℕ) : Nodup (enter_queue e s) := by
-  have ⟨_, h⟩ := enter_queue_WPrefix e s
-  have h1 := nodup_WPrefix e s
+  have ⟨_, h⟩ := enter_queue_Ws e s
+  have h1 := nodup_Ws e s
   rw [← h] at h1
   exact List.Nodup.of_append_right h1
 
@@ -310,8 +207,8 @@ lemma enter_queue_nodup_elements (h : (enter_queue e s)[k]? = some n) (h1 : i �
   apply List.getElem?_inj at h3
   · tauto
   · grind
-  · have ⟨_, h⟩ := enter_queue_WPrefix e s
-    have h1 := nodup_WPrefix e s
+  · have ⟨_, h⟩ := enter_queue_Ws e s
+    have h1 := nodup_Ws e s
     rw [← h] at h1
     exact List.Nodup.of_append_right h1
 
@@ -393,10 +290,12 @@ lemma enter_queue_enum_exact (h : List.idxOf? n (enter_queue e s) = some k) :
 Note that this is *not* the stage at which ϕ_e(n)↓, as n may wait in the enter_queue. -/
 def enum_stage (e n : ℕ) : Part ℕ := Nat.rfind (fun s => (new_element e s == some n))
 
+@[simp]
 lemma enum_stage_spec (s : ℕ) (h : s ∈ enum_stage e n) : new_element e s == some n := by
   have h1 := rfind_spec h
   simp_all only [Part.coe_some, Part.mem_some_iff, Bool.true_eq, beq_iff_eq, BEq.rfl]
 
+@[simp]
 lemma enum_stage_min (s t : ℕ) (h : s ∈ enum_stage e n) (ht : t < s) :
     ¬ (new_element e t == some n) := by
   simp_all only [enum_stage, Part.coe_some, mem_rfind, Part.mem_some_iff, Bool.true_eq, beq_iff_eq,
@@ -429,21 +328,12 @@ lemma enter_queue_exit_exact (h : List.idxOf? n (enter_queue e s) = some k) :
     ∀ t, n ∉ enter_queue e (s + k + t + 1) := by
   intro t
   have h1 := enter_queue_halts (idxOf?_mem (id (Eq.symm h)))
-  have ⟨r, h2⟩ := ϕ_halts_runtime_exists.mp (ϕ_complete.mpr
-    (Exists.intro s h1))
-  apply (ϕNew_runtime_iff e n r).mpr at h2
-  have h3 : r ≤ s := by
-    simp only [ϕNew_runtime_iff] at h2
-    apply runtime_min at h2
-    contrapose h2
-    push Not
-    apply not_le.mp at h2
-    use s
+  replace ⟨r, h2⟩ := runtime_min' h1
+  have h3 : r ≤ s := h2.right
   have h4 : ∀ i, Disjoint (ϕNew e r) (ϕNew e (s+k+1+i)) := by
     intro i
-    refine Disjoint.symm (ϕNew_disjoint_gt ?_)
+    apply ϕNew_pairwise_disjoint
     linarith
-  simp [Finset.disjoint_left] at h4
   induction t with | zero | succ t ih
   <;> nth_rw 1 [enter_queue]
   <;> simp only [mem_append, not_or]
@@ -454,13 +344,14 @@ lemma enter_queue_exit_exact (h : List.idxOf? n (enter_queue e s) = some k) :
         have h6 := enter_queue_enum_exact h
         unfold new_element at h6
         simp_all only [nodup_cons, head?_cons, Option.some.injEq, tail_cons, not_false_eq_true]
-    · simp only [Finset.mem_sort]
-      exact h4 0 h2
+    · exact h4 0 ((ϕNew_runtime e n r).mpr h2.left)
   · constructor
     · contrapose ih
       exact mem_of_mem_tail ih
-    · apply (h4 (t+1)) at h2
+    · rw [← ϕNew_runtime] at h2
+      have h5 := (h4 (t+1)) h2.left
       simp_all [Nat.add_right_comm (s + k) 1 (t + 1)]
+
 
 /- If n is in a queue, eventually it is never in a queue again -/
 lemma enter_queue_exit (h : n ∈ (enter_queue e s)) :
@@ -495,9 +386,11 @@ instance Wenum_dec (e : ℕ) : DecidablePred (fun k => ∃ s, Wenum e k = some s
   simp only [h (enter_queue e n), ne_eq]
   exact instDecidableNot
 
-instance Wenum_comp : Computable (Wenum e)  := by
+instance Wenum_primrec : Primrec (Wenum e)  := by
   unfold Wenum new_element
-  refine Computable.comp (Primrec.to_comp Primrec.list_head?) (enter_queue_comp e)
+  refine Primrec.comp (Primrec.list_head?) (enter_queue_primrec e)
+
+instance Wenum_comp : Computable (Wenum e) := Primrec.to_comp Wenum_primrec
 
 lemma ϕ_halts_Wenum (e n : ℕ) : ϕ_halts e n ↔ ∃ s, n = Wenum e s := by
   rw [← enter_queue_mem]
@@ -514,17 +407,17 @@ lemma ϕ_halts_Wenum (e n : ℕ) : ϕ_halts e n ↔ ∃ s, n = Wenum e s := by
 /-- TODO : extract frequent lemmas? -/
 theorem We_mem_TFAE (e n : ℕ) :
     [n ∈ W e,                  --1
-     ∃ s, n ∈ W_s e s,         --2
+     ∃ s, n ∈ Ws e s,         --2
      ϕ_halts e n,              --3
      ∃ s, n = Wenum e s,       --4
-     ∃ s, ϕ_s_halts e s n,     --5
+     ∃ s, ϕs_halts e s n,     --5
     ].TFAE := by
-  tfae_have 1 ↔ 2 := W_mem_iff_W_s
+  tfae_have 1 ↔ 2 := W_iff_Ws
   tfae_have 3 ↔ 4 := ϕ_halts_Wenum e n
   tfae_have 2 ↔ 5 := by
     apply exists_congr
     intro a
-    exact W_s_ϕ_s
+    exact Ws_mem
   tfae_have 3 ↔ 5 := ϕ_complete
   tfae_finish
 
@@ -548,20 +441,17 @@ lemma queue_depletes (h : (W e).Finite) :
       linarith
     grind
   have hs : s ≥ t := by linarith
-  have hs1 := enter_queue_ϕNewList e hs
-  have hi1 : ∀ i, ϕNewList e (t+i+1) = [] := by
+  have hs1 := enter_queue_ϕNew e hs
+  have hi1 : ∀ i, ϕNew e (t+i+1) = [] := by
     intro i
-    rw [← toFinset_eq_empty_iff]
-    unfold ϕNewList
-    simp
-    grind
+    apply h
+    omega
   simp_all only [gt_iff_lt, ge_iff_le, map_const', length_range, flatten_replicate_nil, append_nil]
   rw [← toFinset_eq_empty_iff]
   ext x
   simp only [mem_toFinset, Finset.notMem_empty, iff_false]
   grind
 
-/-- TODO: the deepest case of this proof is truly horrible, and reused below. Extract! Fix!-/
 lemma Wenum_finite_iff (e : ℕ) : (W e).Finite ↔ ∃ s, ∀ t ≥ s, Wenum e t = Option.none := by
   constructor
   · intro h
@@ -579,15 +469,8 @@ lemma Wenum_finite_iff (e : ℕ) : (W e).Finite ↔ ∃ s, ∀ t ≥ s, Wenum e 
       exact le_of_succ_le h1
     cases s with | zero | succ s
     · tauto
-    · unfold enter_queue at h2
-      simp only [append_eq_nil_iff] at h2
-      obtain ⟨h2, h3⟩ := h2
-      apply Finset.eq_empty_iff_forall_notMem.mpr
-      intro a ha
-      have : a ∈ (ϕNew e (s + 1)).sort (fun a b ↦ a ≤ b) := by
-        exact (Finset.mem_sort fun a b ↦ a ≤ b).mpr ha
-      contrapose h3
-      exact ne_nil_of_mem this
+    · exact (append_eq_nil_iff.mp h2).right
+
 
 
 lemma Wenum_infinite_iff (e : ℕ) : (W e).Infinite ↔ ∀ s, ∃ t ≥ s, ∃ n, Wenum e t = some n := by
@@ -607,58 +490,51 @@ lemma queue_depletes_implies_ϕNew_stabilizes (h : ∃ t, ∀ s ≥ t, enter_que
     rfl
   · cases s with | zero | succ s
     · tauto
-    · unfold enter_queue at h1
-      simp only [append_eq_nil_iff] at h1
-      obtain ⟨h2, h3⟩ := h1
-      apply Finset.eq_empty_iff_forall_notMem.mpr
-      intro a ha
-      have : a ∈ (ϕNew e (s + 1)).sort (fun a b ↦ a ≤ b) := by
-        exact (Finset.mem_sort fun a b ↦ a ≤ b).mpr ha
-      contrapose h3
-      exact ne_nil_of_mem this
+    · simp only [enter_queue, append_eq_nil_iff] at h1
+      simp only [h1, empty_eq]
 
 
-lemma Ws_stabilizes_implies_We_eq_Ws (h : ∃ t, ∀ s ≥ t, W_s e s = W_s e t) :
-    ∃ t, W e = W_s e t := by
+lemma Ws_stabilizes_implies_We_eq_Ws (h : ∃ t, ∀ s ≥ t, Ws e s = Ws e t) :
+    ∃ t, W e = (Ws e t).toFinset := by
   obtain ⟨t, h⟩ := h
   use t
   ext x
-  rw [W_mem_iff_W_s]
+  rw [W_iff_Ws]
   constructor
   <;> intro h1
   · obtain ⟨s, h1⟩ := h1
+    simp only [coe_toFinset, Set.mem_setOf_eq]
     by_cases hts : s > t
-    · grind
-    · exact W_s_mono (Nat.le_of_not_lt hts) h1
+    · replace hts := le_of_succ_le hts
+      simp_all only [ge_iff_le, Std.le_refl, Ws_mem]
+    · push Not at hts
+      exact IsPrefix.mem h1 ((Ws_mono e) hts)
   · grind
 
-lemma We_finite_iff_We_eq_Ws (h : ∃ t, W e = W_s e t) : (W e).Finite := by
+lemma We_finite_iff_We_eq_Ws (h : ∃ t, W e = (Ws e t).toFinset) : (W e).Finite := by
   obtain ⟨t, h⟩ := h
   rw [h]
-  exact Finset.finite_toSet (W_s e t)
+  exact Finset.finite_toSet (Ws e t).toFinset
 
 lemma WsNew_stabilizes_Ws_stabilizes (e : ℕ) (h : ∃ t, ∀ s ≥ t, ϕNew e s = ∅) :
-    ∃ t, ∀ s ≥ t, W_s e s = W_s e t := by
+    ∃ t, ∀ s ≥ t, Ws e s = Ws e t := by
   obtain ⟨t, h⟩ := h
   use t
   intro s
-  have h1 : ∀ s ≥ t, W_s e s = W_s e (s-1) := by
+  have h1 : ∀ s ≥ t, Ws e s = Ws e (s-1) := by
     intro s h1
     induction s with | zero | succ s ih
     · tauto
-    · simp only [add_tsub_cancel_right]
-      apply h at h1
-      rw [ϕNew_eq_Ws_diff] at h1
-      simp only [add_tsub_cancel_right, Finset.sdiff_eq_empty_iff_subset] at h1
-      exact subset_antisymm h1 (W_s_mono (Nat.le_add_right s 1))
+    · apply h at h1
+      simp only [add_tsub_cancel_right, Ws, append_right_eq_self, h1, empty_eq]
   induction s with | zero | succ s ih
   <;> grind
 
 theorem We_finite_TFAE (e : ℕ) :
     [(W e).Finite,                          --1
       ∃ t, ∀ s ≥ t, ϕNew e s = ∅,           --2
-      ∃ t, ∀ s ≥ t, W_s e s = W_s e t,      --3
-      ∃ t, W e = W_s e t,                   --4
+      ∃ t, ∀ s ≥ t, Ws e s = Ws e t,      --3
+      ∃ t, W e = (Ws e t).toFinset,                   --4
       ∃ t, ∀ s ≥ t, enter_queue e s = [],   --5
       ∃ t, ∀ s ≥ t, Wenum e s = Option.none --6
     ].TFAE := by
@@ -673,13 +549,13 @@ theorem We_finite_TFAE (e : ℕ) :
 theorem We_infinite_TFAE (e : ℕ) :
     [(W e).Infinite,                         --1
       ∀ t, ∃ s ≥ t, ϕNew e s ≠ ∅,        --2
-      ∀ t, ∃ s ≥ t, W_s e s ≠ W_s e t,       --3
-      ∀ t, W e ≠ W_s e t,                    --4
+      ∀ t, ∃ s ≥ t, Ws e s ≠ Ws e t,       --3
+      ∀ t, W e ≠ (Ws e t).toFinset,                    --4
       ∀ t, ∃ s ≥ t, enter_queue e s ≠ [],   --5
       ∀ t, ∃ s ≥ t, ∃ n, Wenum e s = some n  --6
     ].TFAE := by
     have h := tfae_not_iff.mpr (We_finite_TFAE e)
     simp only [map] at h
     push Not at h
-    simp only [Finset.nonempty_iff_ne_empty, Option.ne_none_iff_exists'] at h
+    simp only [Option.ne_none_iff_exists'] at h
     exact h
